Rename seal lemmas from `_eq` to `_unseal` and make sealing stuff `Local`.
Also fix some places where we break the seal.

iris/algebra/big_op.v
@@ -35,12 +35,13 @@ Notation "'[^' o 'list]' x ∈ l , P" := (big_opL o (λ _ x, P) l)
   (at level 200, o at level 1, l at level 10, x at level 1, right associativity,
    format "[^ o  list]  x  ∈  l ,  P") : stdpp_scope.
 
-Definition big_opM_def `{Monoid M o} `{Countable K} {A} (f : K → A → M)
+Local Definition big_opM_def `{Monoid M o} `{Countable K} {A} (f : K → A → M)
   (m : gmap K A) : M := big_opL o (λ _, uncurry f) (map_to_list m).
-Definition big_opM_aux : seal (@big_opM_def). Proof. by eexists. Qed.
+Local Definition big_opM_aux : seal (@big_opM_def). Proof. by eexists. Qed.
 Definition big_opM := big_opM_aux.(unseal).
 Global Arguments big_opM {M} o {_ K _ _ A} _ _.
-Definition big_opM_eq : @big_opM = @big_opM_def := big_opM_aux.(seal_eq).
+Local Definition big_opM_unseal :
+  @big_opM = @big_opM_def := big_opM_aux.(seal_eq).
 Global Instance: Params (@big_opM) 7 := {}.
 Notation "'[^' o 'map]' k ↦ x ∈ m , P" := (big_opM o (λ k x, P) m)
   (at level 200, o at level 1, m at level 10, k, x at level 1, right associativity,
@@ -49,23 +50,25 @@ Notation "'[^' o 'map]' x ∈ m , P" := (big_opM o (λ _ x, P) m)
   (at level 200, o at level 1, m at level 10, x at level 1, right associativity,
    format "[^ o  map]  x  ∈  m ,  P") : stdpp_scope.
 
-Definition big_opS_def `{Monoid M o} `{Countable A} (f : A → M)
+Local Definition big_opS_def `{Monoid M o} `{Countable A} (f : A → M)
   (X : gset A) : M := big_opL o (λ _, f) (elements X).
-Definition big_opS_aux : seal (@big_opS_def). Proof. by eexists. Qed.
+Local Definition big_opS_aux : seal (@big_opS_def). Proof. by eexists. Qed.
 Definition big_opS := big_opS_aux.(unseal).
 Global Arguments big_opS {M} o {_ A _ _} _ _.
-Definition big_opS_eq : @big_opS = @big_opS_def := big_opS_aux.(seal_eq).
+Local Definition big_opS_unseal :
+  @big_opS = @big_opS_def := big_opS_aux.(seal_eq).
 Global Instance: Params (@big_opS) 6 := {}.
 Notation "'[^' o 'set]' x ∈ X , P" := (big_opS o (λ x, P) X)
   (at level 200, o at level 1, X at level 10, x at level 1, right associativity,
    format "[^ o  set]  x  ∈  X ,  P") : stdpp_scope.
 
-Definition big_opMS_def `{Monoid M o} `{Countable A} (f : A → M)
+Local Definition big_opMS_def `{Monoid M o} `{Countable A} (f : A → M)
   (X : gmultiset A) : M := big_opL o (λ _, f) (elements X).
-Definition big_opMS_aux : seal (@big_opMS_def). Proof. by eexists. Qed.
+Local Definition big_opMS_aux : seal (@big_opMS_def). Proof. by eexists. Qed.
 Definition big_opMS := big_opMS_aux.(unseal).
 Global Arguments big_opMS {M} o {_ A _ _} _ _.
-Definition big_opMS_eq : @big_opMS = @big_opMS_def := big_opMS_aux.(seal_eq).
+Local Definition big_opMS_unseal :
+  @big_opMS = @big_opMS_def := big_opMS_aux.(seal_eq).
 Global Instance: Params (@big_opMS) 6 := {}.
 Notation "'[^' o 'mset]' x ∈ X , P" := (big_opMS o (λ x, P) X)
   (at level 200, o at level 1, X at level 10, x at level 1, right associativity,
@@ -252,12 +255,12 @@ Proof. by apply big_opL_sep_zip_with. Qed.
 
 Lemma big_opM_empty `{Countable K} {B} (f : K → B → M) :
   ([^o map] k↦x ∈ ∅, f k x) = monoid_unit.
-Proof. by rewrite big_opM_eq /big_opM_def map_to_list_empty. Qed.
+Proof. by rewrite big_opM_unseal /big_opM_def map_to_list_empty. Qed.
 
 Lemma big_opM_insert `{Countable K} {B} (f : K → B → M) (m : gmap K B) i x :
   m !! i = None →
   ([^o map] k↦y ∈ <[i:=x]> m, f k y) ≡ f i x `o` [^o map] k↦y ∈ m, f k y.
-Proof. intros ?. by rewrite big_opM_eq /big_opM_def map_to_list_insert. Qed.
+Proof. intros ?. by rewrite big_opM_unseal /big_opM_def map_to_list_insert. Qed.
 
 Lemma big_opM_delete `{Countable K} {B} (f : K → B → M) (m : gmap K B) i x :
   m !! i = Some x →
@@ -304,7 +307,7 @@ Section gmap.
     (∀ k x, m !! k = Some x → R (f k x) (g k x)) →
     R ([^o map] k ↦ x ∈ m, f k x) ([^o map] k ↦ x ∈ m, g k x).
   Proof.
-    intros ?? Hf. rewrite big_opM_eq. apply (big_opL_gen_proper R); auto.
+    intros ?? Hf. rewrite big_opM_unseal. apply (big_opL_gen_proper R); auto.
     intros k [i x] ?%elem_of_list_lookup_2. by apply Hf, elem_of_map_to_list.
   Qed.
 
@@ -353,7 +356,7 @@ Section gmap.
   [setoid_rewrite] in the proof of [big_sepS_sepS]. See Coq issue #14349. *)
   Lemma big_opM_map_to_list f m :
     ([^o map] k↦x ∈ m, f k x) ≡ [^o list] xk ∈ map_to_list m, f (xk.1) (xk.2).
-  Proof. rewrite big_opM_eq. apply big_opL_proper'; [|done]. by intros ? [??]. Qed.
+  Proof. rewrite big_opM_unseal. apply big_opL_proper'; [|done]. by intros ? [??]. Qed.
 
   Lemma big_opM_singleton f i x : ([^o map] k↦y ∈ {[i:=x]}, f k y) ≡ f i x.
   Proof.
@@ -363,13 +366,13 @@ Section gmap.
 
   Lemma big_opM_unit m : ([^o map] k↦y ∈ m, monoid_unit) ≡ (monoid_unit : M).
   Proof.
-    by induction m using map_ind; rewrite /= ?big_opM_insert ?left_id // big_opM_eq.
+    by induction m using map_ind; rewrite /= ?big_opM_insert ?left_id // big_opM_unseal.
   Qed.
 
   Lemma big_opM_fmap {B} (h : A → B) (f : K → B → M) m :
     ([^o map] k↦y ∈ h <$> m, f k y) ≡ ([^o map] k↦y ∈ m, f k (h y)).
   Proof.
-    rewrite big_opM_eq /big_opM_def map_to_list_fmap big_opL_fmap.
+    rewrite big_opM_unseal /big_opM_def map_to_list_fmap big_opL_fmap.
     by apply big_opL_proper=> ? [??].
   Qed.
 
@@ -445,7 +448,7 @@ Section gmap.
     ([^o map] k↦x ∈ m, f k x `o` g k x)
     ≡ ([^o map] k↦x ∈ m, f k x) `o` ([^o map] k↦x ∈ m, g k x).
   Proof.
-    rewrite big_opM_eq /big_opM_def -big_opL_op. by apply big_opL_proper=> ? [??].
+    rewrite big_opM_unseal /big_opM_def -big_opL_op. by apply big_opL_proper=> ? [??].
   Qed.
 End gmap.
 
@@ -483,7 +486,7 @@ Section gset.
     (∀ x, x ∈ X → R (f x) (g x)) →
     R ([^o set] x ∈ X, f x) ([^o set] x ∈ X, g x).
   Proof.
-    rewrite big_opS_eq. intros ?? Hf. apply (big_opL_gen_proper R); auto.
+    rewrite big_opS_unseal. intros ?? Hf. apply (big_opL_gen_proper R); auto.
     intros k x ?%elem_of_list_lookup_2. by apply Hf, elem_of_elements.
   Qed.
 
@@ -514,10 +517,10 @@ Section gset.
   [setoid_rewrite] in the proof of [big_sepS_sepS]. See Coq issue #14349. *)
   Lemma big_opS_elements f X :
     ([^o set] x ∈ X, f x) ≡ [^o list] x ∈ elements X, f x.
-  Proof. by rewrite big_opS_eq. Qed.
+  Proof. by rewrite big_opS_unseal. Qed.
 
   Lemma big_opS_empty f : ([^o set] x ∈ ∅, f x) = monoid_unit.
-  Proof. by rewrite big_opS_eq /big_opS_def elements_empty. Qed.
+  Proof. by rewrite big_opS_unseal /big_opS_def elements_empty. Qed.
 
   Lemma big_opS_insert f X x :
     x ∉ X → ([^o set] y ∈ {[ x ]} ∪ X, f y) ≡ (f x `o` [^o set] y ∈ X, f y).
@@ -557,7 +560,7 @@ Section gset.
 
   Lemma big_opS_unit X : ([^o set] y ∈ X, monoid_unit) ≡ (monoid_unit : M).
   Proof.
-    by induction X using set_ind_L; rewrite /= ?big_opS_insert ?left_id // big_opS_eq.
+    by induction X using set_ind_L; rewrite /= ?big_opS_insert ?left_id // big_opS_unseal.
   Qed.
 
   Lemma big_opS_filter' (φ : A → Prop) `{∀ x, Decision (φ x)} f X :
@@ -605,7 +608,7 @@ Lemma big_opM_dom `{Countable K} {A} (f : K → M) (m : gmap K A) :
   ([^o map] k↦_ ∈ m, f k) ≡ ([^o set] k ∈ dom m, f k).
 Proof.
   induction m as [|i x ?? IH] using map_ind.
-  { by rewrite big_opM_eq big_opS_eq dom_empty_L. }
+  { by rewrite big_opM_unseal big_opS_unseal dom_empty_L. }
   by rewrite dom_insert_L big_opM_insert // IH big_opS_insert ?not_elem_of_dom.
 Qed.
 
@@ -620,7 +623,7 @@ Section gmultiset.
     (∀ x, x ∈ X → R (f x) (g x)) →
     R ([^o mset] x ∈ X, f x) ([^o mset] x ∈ X, g x).
   Proof.
-    rewrite big_opMS_eq. intros ?? Hf. apply (big_opL_gen_proper R); auto.
+    rewrite big_opMS_unseal. intros ?? Hf. apply (big_opL_gen_proper R); auto.
     intros k x ?%elem_of_list_lookup_2. by apply Hf, gmultiset_elem_of_elements.
   Qed.
 
@@ -651,18 +654,18 @@ Section gmultiset.
   [setoid_rewrite] in the proof of [big_sepS_sepS]. See Coq issue #14349. *)
   Lemma big_opMS_elements f X :
     ([^o mset] x ∈ X, f x) ≡ [^o list] x ∈ elements X, f x.
-  Proof. by rewrite big_opMS_eq. Qed.
+  Proof. by rewrite big_opMS_unseal. Qed.
 
   Lemma big_opMS_empty f : ([^o mset] x ∈ ∅, f x) = monoid_unit.
-  Proof. by rewrite big_opMS_eq /big_opMS_def gmultiset_elements_empty. Qed.
+  Proof. by rewrite big_opMS_unseal /big_opMS_def gmultiset_elements_empty. Qed.
 
   Lemma big_opMS_disj_union f X Y :
     ([^o mset] y ∈ X ⊎ Y, f y) ≡ ([^o mset] y ∈ X, f y) `o` [^o mset] y ∈ Y, f y.
-  Proof. by rewrite big_opMS_eq /big_opMS_def gmultiset_elements_disj_union big_opL_app. Qed.
+  Proof. by rewrite big_opMS_unseal /big_opMS_def gmultiset_elements_disj_union big_opL_app. Qed.
 
   Lemma big_opMS_singleton f x : ([^o mset] y ∈ {[+ x +]}, f y) ≡ f x.
   Proof.
-    intros. by rewrite big_opMS_eq /big_opMS_def gmultiset_elements_singleton /= right_id.
+    intros. by rewrite big_opMS_unseal /big_opMS_def gmultiset_elements_singleton /= right_id.
   Qed.
 
   Lemma big_opMS_insert f X x :
@@ -679,12 +682,12 @@ Section gmultiset.
   Lemma big_opMS_unit X : ([^o mset] y ∈ X, monoid_unit) ≡ (monoid_unit : M).
   Proof.
     by induction X using gmultiset_ind;
-      rewrite /= ?big_opMS_disj_union ?big_opMS_singleton ?left_id // big_opMS_eq.
+      rewrite /= ?big_opMS_disj_union ?big_opMS_singleton ?left_id // big_opMS_unseal.
   Qed.
 
   Lemma big_opMS_op f g X :
     ([^o mset] y ∈ X, f y `o` g y) ≡ ([^o mset] y ∈ X, f y) `o` ([^o mset] y ∈ X, g y).
-  Proof. by rewrite big_opMS_eq /big_opMS_def -big_opL_op. Qed.
+  Proof. by rewrite big_opMS_unseal /big_opMS_def -big_opL_op. Qed.
 End gmultiset.
 
 (** Commuting lemmas *)
