iris/base_logic/lib/fancy_updates.v
@@ -7,54 +7,56 @@ From iris.prelude Require Import options.
 Export invGS.
 Import uPred.
 
-Definition uPred_fupd_def `{!invGS Σ} (E1 E2 : coPset) (P : iProp Σ) : iProp Σ :=
+Local Definition uPred_fupd_def `{!invGS Σ} (E1 E2 : coPset) (P : iProp Σ) : iProp Σ :=
   wsat ∗ ownE E1 ==∗ ◇ (wsat ∗ ownE E2 ∗ P).
-Definition uPred_fupd_aux : seal (@uPred_fupd_def). Proof. by eexists. Qed.
+Local Definition uPred_fupd_aux : seal (@uPred_fupd_def). Proof. by eexists. Qed.
 Definition uPred_fupd := uPred_fupd_aux.(unseal).
 Global Arguments uPred_fupd {Σ _}.
-Lemma uPred_fupd_eq `{!invGS Σ} : @fupd _ uPred_fupd = uPred_fupd_def.
+Local Lemma uPred_fupd_unseal `{!invGS Σ} : @fupd _ uPred_fupd = uPred_fupd_def.
 Proof. rewrite -uPred_fupd_aux.(seal_eq) //. Qed.
 
 Lemma uPred_fupd_mixin `{!invGS Σ} : BiFUpdMixin (uPredI (iResUR Σ)) uPred_fupd.
 Proof.
   split.
-  - rewrite uPred_fupd_eq. solve_proper.
+  - rewrite uPred_fupd_unseal. solve_proper.
   - intros E1 E2 (E1''&->&?)%subseteq_disjoint_union_L.
-    rewrite uPred_fupd_eq /uPred_fupd_def ownE_op //.
+    rewrite uPred_fupd_unseal /uPred_fupd_def ownE_op //.
     by iIntros "($ & $ & HE) !> !> [$ $] !> !>" .
-  - rewrite uPred_fupd_eq. iIntros (E1 E2 P) ">H [Hw HE]". iApply "H"; by iFrame.
-  - rewrite uPred_fupd_eq. iIntros (E1 E2 P Q HPQ) "HP HwE". rewrite -HPQ. by iApply "HP".
-  - rewrite uPred_fupd_eq. iIntros (E1 E2 E3 P) "HP HwE".
+  - rewrite uPred_fupd_unseal.
+    iIntros (E1 E2 P) ">H [Hw HE]". iApply "H"; by iFrame.
+  - rewrite uPred_fupd_unseal.
+    iIntros (E1 E2 P Q HPQ) "HP HwE". rewrite -HPQ. by iApply "HP".
+  - rewrite uPred_fupd_unseal. iIntros (E1 E2 E3 P) "HP HwE".
     iMod ("HP" with "HwE") as ">(Hw & HE & HP)". iApply "HP"; by iFrame.
-  - intros E1 E2 Ef P HE1Ef. rewrite uPred_fupd_eq /uPred_fupd_def ownE_op //.
+  - intros E1 E2 Ef P HE1Ef. rewrite uPred_fupd_unseal /uPred_fupd_def ownE_op //.
     iIntros "Hvs (Hw & HE1 &HEf)".
     iMod ("Hvs" with "[Hw HE1]") as ">($ & HE2 & HP)"; first by iFrame.
     iDestruct (ownE_op' with "[HE2 HEf]") as "[? $]"; first by iFrame.
     iIntros "!> !>". by iApply "HP".
-  - rewrite uPred_fupd_eq /uPred_fupd_def. by iIntros (????) "[HwP $]".
+  - rewrite uPred_fupd_unseal /uPred_fupd_def. by iIntros (????) "[HwP $]".
 Qed.
 Global Instance uPred_bi_fupd `{!invGS Σ} : BiFUpd (uPredI (iResUR Σ)) :=
   {| bi_fupd_mixin := uPred_fupd_mixin |}.
 
 Global Instance uPred_bi_bupd_fupd `{!invGS Σ} : BiBUpdFUpd (uPredI (iResUR Σ)).
-Proof. rewrite /BiBUpdFUpd uPred_fupd_eq. by iIntros (E P) ">? [$ $] !> !>". Qed.
+Proof. rewrite /BiBUpdFUpd uPred_fupd_unseal. by iIntros (E P) ">? [$ $] !> !>". Qed.
 
 Global Instance uPred_bi_fupd_plainly `{!invGS Σ} : BiFUpdPlainly (uPredI (iResUR Σ)).
 Proof.
   split.
-  - rewrite uPred_fupd_eq /uPred_fupd_def. iIntros (E P) "H [Hw HE]".
+  - rewrite uPred_fupd_unseal /uPred_fupd_def. iIntros (E P) "H [Hw HE]".
     iAssert (◇ ■ P)%I as "#>HP".
     { by iMod ("H" with "[$]") as "(_ & _ & HP)". }
     by iFrame.
-  - rewrite uPred_fupd_eq /uPred_fupd_def. iIntros (E P Q) "[H HQ] [Hw HE]".
+  - rewrite uPred_fupd_unseal /uPred_fupd_def. iIntros (E P Q) "[H HQ] [Hw HE]".
     iAssert (◇ ■ P)%I as "#>HP".
     { by iMod ("H" with "HQ [$]") as "(_ & _ & HP)". }
     by iFrame.
-  - rewrite uPred_fupd_eq /uPred_fupd_def. iIntros (E P) "H [Hw HE]".
+  - rewrite uPred_fupd_unseal /uPred_fupd_def. iIntros (E P) "H [Hw HE]".
     iAssert (▷ ◇ ■ P)%I as "#HP".
     { iNext. by iMod ("H" with "[$]") as "(_ & _ & HP)". }
     iFrame. iIntros "!> !> !>". by iMod "HP".
-  - rewrite uPred_fupd_eq /uPred_fupd_def. iIntros (E A Φ) "HΦ [Hw HE]".
+  - rewrite uPred_fupd_unseal /uPred_fupd_def. iIntros (E A Φ) "HΦ [Hw HE]".
     iAssert (◇ ■ ∀ x : A, Φ x)%I as "#>HP".
     { iIntros (x). by iMod ("HΦ" with "[$Hw $HE]") as "(_&_&?)". }
     by iFrame.
@@ -66,7 +68,7 @@ Proof.
   iIntros (Hfupd). apply later_soundness. iMod wsat_alloc as (Hinv) "[Hw HE]".
   iAssert (|={⊤,E2}=> P)%I as "H".
   { iMod (fupd_mask_subseteq E1) as "_"; first done. iApply Hfupd. }
-  rewrite uPred_fupd_eq /uPred_fupd_def.
+  rewrite uPred_fupd_unseal /uPred_fupd_def.
   iMod ("H" with "[$]") as "[Hw [HE >H']]"; iFrame.
 Qed.
 
